split files into fst and fsti

intermediate/Veritas.Intermediate.Logs.fst
@@ -1,28 +1,22 @@
 module Veritas.Intermediate.Logs
 
-module K = Veritas.Key
-module MHD = Veritas.MultiSetHashDomain
-module R = Veritas.Record
-module SA = Veritas.SeqAux
-module V = Veritas.Verifier
+open Veritas.Key
+open Veritas.MultiSetHashDomain
+open Veritas.Record
+open Veritas.SeqAux
+open Veritas.Intermediate.StoreSKC
 
-let slot_id = Veritas.Intermediate.Store.slot_id
-let key = K.key
-let data_key = K.data_key
-let merkle_key = K.merkle_key
-let value = R.value
-let data_value = R.data_value
-let record = R.record
-let timestamp = MHD.timestamp
-let thread_id = V.thread_id
+module Spec = Veritas.Verifier
+
+let thread_id = Spec.thread_id
 
 (* Definitions of different styles of verifier logs.
    - logK : contains only key references (defined in Veritas.Verifier)
    - logSK: contains both slot and key references
    - logS: contains only slot references *)
 
-let logK_entry = V.vlog_entry
-let logK = V.vlog
+let logK_entry = Spec.vlog_entry
+let logK = Spec.vlog
 
 noeq
 type logSK_entry =
@@ -50,16 +44,16 @@ let logS = Seq.seq logS_entry
 
 let drop_slots_aux (e:logSK_entry) :logK_entry =
   match e with
-  | Get_SK _ k v -> V.Get k v
-  | Put_SK _ k v -> V.Put k v
-  | AddM_SK _ r _ k' -> V.AddM r k'
-  | EvictM_SK _ k _ k' -> V.EvictM k k'
-  | AddB_SK _ r t j -> V.AddB r t j
-  | EvictB_SK _ k t -> V.EvictB k t
-  | EvictBM_SK _ k _ k' t -> V.EvictBM k k' t
+  | Get_SK _ k v -> Spec.Get k v
+  | Put_SK _ k v -> Spec.Put k v
+  | AddM_SK _ r _ k' -> Spec.AddM r k'
+  | EvictM_SK _ k _ k' -> Spec.EvictM k k'
+  | AddB_SK _ r t j -> Spec.AddB r t j
+  | EvictB_SK _ k t -> Spec.EvictB k t
+  | EvictBM_SK _ k _ k' t -> Spec.EvictBM k k' t
   
 let drop_slots (l:logSK) : logK 
-  = SA.map drop_slots_aux l
+  = map drop_slots_aux l
 
 // likely similar to EAC: check that for every "OP s k ...", k is the last key added at slot s, and has not been evicted 
 let skc (l:logSK) : Type = admit()
