intermediate/Veritas.Intermediate.VerifySKC.fst
@@ -1,392 +1,235 @@
 module Veritas.Intermediate.VerifySKC
-open Veritas.Intermediate.Logs
-open Veritas.Intermediate.Store
 
-module BT = Veritas.BinTree
-module FE = FStar.FunctionalExtensionality
-module H = Veritas.Hash
-module K = Veritas.Key
-module MH = Veritas.MultiSetHash
-module MHD = Veritas.MultiSetHashDomain
-module R = Veritas.Record
-module SA = Veritas.SeqAux
-module V = Veritas.Verifier
-module VT = Veritas.Verifier.Thread
-
-let data_key = K.data_key
-let merkle_key = K.merkle_key
-let data_value = R.data_value 
-let thread_id = V.thread_id
-let timestamp = MHD.timestamp
-
-(* Thread-local state
-   id     : thread id
-   st     : thread local store
-   clock  : current timestamp
-   hadd   : add set hash
-   hevict : evict set hash *)
-noeq
-type vtls =
-  | Failed : vtls
-  | Valid :
-    id : thread_id ->
-    st : vstore ->
-    clock : timestamp ->
-    hadd : MH.ms_hash_value ->
-    hevict : MH.ms_hash_value ->
-    vtls
-
-let thread_id_of (vs:vtls {Valid? vs}): thread_id = 
-  Valid?.id vs
-
-let thread_store (vs: vtls {Valid? vs}): vstore =
-  Valid?.st vs
-
-let thread_store_is_map (vs: vtls {Valid? vs}): bool =
-  let st = thread_store vs in st.is_map
-
-let update_thread_store (vs:vtls {Valid? vs}) (st:vstore) : vtls =
-  match vs with
-  | Valid id _ clock hadd hevict -> Valid id st clock hadd hevict
-
-let thread_clock (vs:vtls {Valid? vs}) = 
-  Valid?.clock vs
-
-let update_thread_clock (vs:vtls {Valid? vs}) (clock:timestamp): vtls = 
-  match vs with
-  | Valid id st _ hadd hevict -> Valid id st clock hadd hevict
-
-let thread_hadd (vs:vtls {Valid? vs}) = 
-  Valid?.hadd vs
-
-let thread_hevict (vs:vtls {Valid? vs}) = 
-  Valid?.hevict vs
-
-let update_thread_hadd (vs:vtls {Valid? vs}) (hadd: MH.ms_hash_value): vtls = 
-  match vs with
-  | Valid id st clock _ hevict -> Valid id st clock hadd hevict
-
-let update_thread_hevict (vs:vtls {Valid? vs}) (hevict:MH.ms_hash_value): vtls = 
-  match vs with
-  | Valid id st clock hadd _ -> Valid id st clock hadd hevict
-
-let vget (s:slot_id) (k:data_key) (v:data_value) (vs: vtls {Valid? vs}) : vtls =
+let vget (s:slot_id) (v:data_value) (vs: vtls {Valid? vs}) : vtls =
   let st = thread_store vs in
   (* check store contains slot s *)
-  if not (contains_record st s) then Failed
+  if not (store_contains st s) then Failed
   (* check stored key and value *)
-  else let k' = get_key_at st s in
-       let v' = get_value_at st s in
-       if k' <> k then Failed
-       else if not (R.DVal? v') then Failed
-       else if R.to_data_value v' <> v then Failed
+  else let v' = stored_value st s in
+       if not (DVal? v') then Failed
+       else if to_data_value v' <> v then Failed
        else vs
 
-let vput (s:slot_id) (k:data_key) (v:data_value) (vs: vtls {Valid? vs}) : vtls =
+let vput (s:slot_id) (v:data_value) (vs: vtls {Valid? vs}) : vtls =
   let st = thread_store vs in
   (* check store contains slot s *)
-  if not (contains_record st s) then Failed
+  if not (store_contains st s) then Failed
   (* check stored key is k *)
-  else if get_key_at st s <> k then Failed
-  else update_thread_store vs (update_record_value st s (R.DVal v))
+  else if not (is_data_key (stored_key st s)) then Failed
+  else update_thread_store vs (update_store st s (DVal v))
 
-let vaddm (s:slot_id) (r:R.record) (s':slot_id) (k0':merkle_key) (vs: vtls {Valid? vs}): vtls =
+let vaddm (s:slot_id) (r:record) (s':slot_id) (vs: vtls {Valid? vs}): vtls =
   let st = thread_store vs in
+  let (k,v) = r in
   if not (s < Seq.length st.data) then Failed
   (* check store contains slot s' *)
-  else if not (contains_record st s') then Failed
+  else if not (store_contains st s') then Failed
   else
-    let (k,v) = r in
-    let k' = get_key_at st s' in
-    let v' = get_value_at st s' in
-    let a' = get_add_method_at st s' in 
-    (* check key is consistent with argument *)
-    if k' <> k0' then Failed
+    let k' = stored_key st s' in
+    let v' = stored_value st s' in
+    let a' = add_method_of st s' in
     (* check k is a proper desc of k' *)
-    else if not (BT.is_proper_desc k k') then Failed
+    if not (is_proper_desc k k') then Failed
     (* check store does not contain slot s *)
-    else if contains_record st s then Failed
+    else if store_contains st s then Failed
+    (* check store does not contain key k
+       >> in lower levels we will check this via 'in_store' fields *)
+    else if store_contains_key st k then Failed
     (* check type of v is consistent with k *)
-    else if not (R.is_value_of k v) then Failed
+    else if not (is_value_of k v) then Failed
     (* check v' is a merkle value *)
-    else if R.DVal? v' then Failed 
+    else if DVal? v' then Failed 
     else
-      let v' = R.to_merkle_value v' in
-      let d = BT.desc_dir k k' in
-      let dh' = R.desc_hash_dir v' d in 
-      (* check k is not already in the store
-         >> in lower levels we will check this via 'in_store' fields in records *)
-      if contains_key st k then Failed
-      else let h = H.hashfn v in
+      let v' = to_merkle_value v' in
+      let d = desc_dir k k' in
+      let dh' = desc_hash_dir v' d in 
+      let h = hashfn v in
       match dh' with
-      | R.Empty -> (* k' has no child in direction d *)
-                (* first add --> init value *)
-                if v <> R.init_value k then Failed
-                else
-                  let v'_upd = V.update_merkle_value v' d k h false in
-                  let st_upd = update_record_value st s' (R.MVal v'_upd) in
-                  let st_upd2 = add_record st_upd s k v V.MAdd in
-                  update_thread_store vs st_upd2
-      | R.Desc k2 h2 b2 -> if k2 = k then
-                          (* k is a child of k' *)
-                          (* check hashes match and k was not evicted to blum *)
-                          if not (h2 = h && b2 = false) then Failed
-                          else update_thread_store vs (add_record st s k v V.MAdd)
-                          (* k is not a child of k' *)
-                          (* first add --> init value *)
-                        else if v <> R.init_value k then Failed
-                        (* check k2 is a proper desc of k *)
-                        else if not (BT.is_proper_desc k2 k) then Failed
-                        else
-                          let d2 = BT.desc_dir k2 k in
-                          let mv = R.to_merkle_value v in
-                          let mv_upd = V.update_merkle_value mv d2 k2 h2 b2 in
-                          let v'_upd = V.update_merkle_value v' d k h false in
-                          let st_upd = update_record_value st s' (R.MVal  v'_upd) in
-                          let st_upd2 = add_record st_upd s k (R.MVal mv_upd) V.MAdd in
-                          update_thread_store vs st_upd2
+      | Empty -> (* k' has no child in direction d *)
+          (* first add must be init value *)
+          if v <> init_value k then Failed
+          else
+            let v'_upd = Spec.update_merkle_value v' d k h false in
+            let st_upd = update_store st s' (MVal v'_upd) in
+            let st_upd2 = add_to_store st_upd s k v Spec.MAdd in
+            update_thread_store vs st_upd2
+      | Desc k2 h2 b2 -> 
+          if k2 = k 
+          then (* k is a child of k' *)
+            (* check hashes match and k was not evicted to blum *)
+            if not (h2 = h && b2 = false) then Failed
+            else update_thread_store vs (add_to_store st s k v Spec.MAdd)
+          else (* otherwise, k is not a child of k' *)
+          (* first add must be init value *)
+          if v <> init_value k then Failed
+          (* check k2 is a proper desc of k *)
+          else if not (is_proper_desc k2 k) then Failed
+          else
+            let d2 = desc_dir k2 k in
+            let mv = to_merkle_value v in
+            let mv_upd = Spec.update_merkle_value mv d2 k2 h2 b2 in
+            let v'_upd = Spec.update_merkle_value v' d k h false in
+            let st_upd = update_store st s' (MVal v'_upd) in
+            let st_upd2 = add_to_store st_upd s k (MVal mv_upd) Spec.MAdd in
+            update_thread_store vs st_upd2
 
 (* key k is in store and was added using Merkle *)
 let is_instore_madd (st: vstore) (k: key): bool = 
-  contains_key st k && 
-  add_method_of st k = V.MAdd
+  store_contains_key st k && 
+  add_method_of_by_key st k = Spec.MAdd
 
-let has_instore_merkle_desc (st:vstore) (k:key{contains_key st k}): bool = 
-  if K.is_data_key k then false
+let has_instore_merkle_desc (st:vstore) (k:key{store_contains_key st k}): bool = 
+  if is_data_key k then false
   else 
-    let v = R.to_merkle_value (value_of st k) in
-    let ld = R.desc_hash_dir v BT.Left in
-    let rd = R.desc_hash_dir v BT.Right in
-    R.Desc? ld && is_instore_madd st (R.Desc?.k ld) || 
-    R.Desc? rd && is_instore_madd st (R.Desc?.k rd)
+    let v = to_merkle_value (stored_value_by_key st k) in
+    let ld = desc_hash_dir v Left in
+    let rd = desc_hash_dir v Right in
+    Desc? ld && is_instore_madd st (Desc?.k ld) || 
+    Desc? rd && is_instore_madd st (Desc?.k rd)
 
-let vevictm (s:slot_id) (k0:key) (s':slot_id) (k0':merkle_key) (vs: vtls {Valid? vs}): vtls = 
+let vevictm (s:slot_id) (s':slot_id) (vs: vtls {Valid? vs}): vtls = 
   let st = thread_store vs in
   (* check store contains s and s' *)
-  if not (contains_record st s && contains_record st s') then Failed
+  if not (store_contains st s && store_contains st s') then Failed
   else 
-    let k = get_key_at st s in
-    let v = get_value_at st s in
-    let a = get_add_method_at st s in
-    let k' = get_key_at st s' in
-    let v' = get_value_at st s' in
-    let a' = get_add_method_at st s' in
-    (* check keys are consistent with arguments *)
-    if k <> k0 then Failed
-    else if k' <> k0' then Failed
+    let k = stored_key st s in
+    let v = stored_value st s in
+    let k' = stored_key st s' in
+    let v' = stored_value st s' in
     (* check k is a proper descendent of k' *)
-    else if not (BT.is_proper_desc k k') then Failed
+    if not (is_proper_desc k k') then Failed
     (* check k does not have a child in the store *)
-    else if (
-              lemma_contains_key st s k; 
-              has_instore_merkle_desc st k
-            ) then Failed
-    else 
-      let d = BT.desc_dir k k' in
-      let v' = R.to_merkle_value v' in
-      let dh' = R.desc_hash_dir v' d in
-      let h = H.hashfn v in
+    else if has_instore_merkle_desc st k then Failed
+    else
+      let d = desc_dir k k' in
+      // TODO: remove the assert with a better SMTPat for stored_value_matches_stored_key
+      let _ = assert (is_value_of k' v') in 
+      let v' = to_merkle_value v' in
+      let dh' = desc_hash_dir v' d in
+      let h = hashfn v in
       match dh' with
-      | R.Empty -> Failed
-      | R.Desc k2 h2 b2 -> if k2 <> k then Failed
-                        else
-                          let v'_upd = V.update_merkle_value v' d k h false in
-                          let st_upd = evict_record (update_record_value st s' (R.MVal v'_upd)) s in
-                         update_thread_store vs st_upd
+      | Empty -> Failed
+      | Desc k2 h2 b2 -> 
+          if k2 <> k then Failed
+          else
+            let v'_upd = Spec.update_merkle_value v' d k h false in
+            let st_upd = update_store st s' (MVal v'_upd) in
+            let st_upd2 = evict_from_store st_upd s in
+            update_thread_store vs st_upd2
 
-let vaddb (s:slot_id) (r:R.record) (t:timestamp) (j:thread_id) (vs:vtls {Valid? vs}): vtls = 
-  let st = thread_store vs in 
-  if not (s < Seq.length st.data) then Failed
+let vaddb (s:slot_id) (r:record) (t:timestamp) (j:thread_id) (vs:vtls {Valid? vs}): vtls = 
   (* epoch of timestamp of last evict *)
+  let e = MkTimestamp?.e t in
+  let st = thread_store vs in 
+  let (k,v) = r in
+  if not (s < Seq.length st.data) then Failed
   else 
-    let e = MHD.MkTimestamp?.e t in
-    let (k,v) = r in
     (* check value type consistent with key k *)
-    if not (R.is_value_of k v) then Failed
+    if not (is_value_of k v) then Failed
     (* check store contains slot s *)
-    else if contains_record st s then Failed
+    else if store_contains st s then Failed
     else 
       (* update add hash *)
       let h = thread_hadd vs in
-      let h_upd = MH.ms_hashfn_upd (MHD.MHDom (k,v) t j) h in
+      let h_upd = ms_hashfn_upd (MHDom (k,v) t j) h in
       let vs_upd = update_thread_hadd vs h_upd in
       (* update clock *)
       let clk = thread_clock vs in
-      let clk_upd = V.max clk (MHD.next t) in
+      let clk_upd = Spec.max clk (next t) in
       let vs_upd2 = update_thread_clock vs_upd clk_upd in
       (* check k is not in the store; update the valid flag accordingly *)
-      let valid = not (contains_key st k) in
-      let st_upd = update_is_map st (st.is_map && valid) in
+      let valid = not (store_contains_key st k) in
+      let st_upd = {st with is_map=(st.is_map && valid)} in
       (* add record to store *)
-      let st_upd2 = add_record st_upd s k v V.BAdd in
+      let st_upd2 = add_to_store st_upd s k v Spec.BAdd in
       update_thread_store vs_upd2 st_upd2
 
-let vevictb (s:slot_id) (k0:key) (t:timestamp) (vs:vtls {Valid? vs}): vtls = 
+let vevictb (s:slot_id) (t:timestamp) (vs:vtls {Valid? vs}): vtls = 
   let clock = thread_clock vs in
-  let e = MHD.MkTimestamp?.e t in
+  let e = MkTimestamp?.e t in
   let st = thread_store vs in
   (* check store contains slot s *)
-  if not (contains_record st s) then Failed
+  if not (store_contains st s) then Failed
   else
-    let k = get_key_at st s in
-    let v = get_value_at st s in
-    (* check key is consistent with argument *)
-    if k <> k0 then Failed
+    let k = stored_key st s in
+    let v = stored_value st s in
     (* check key at s is not root *)
-    else if k = BT.Root then Failed
+    if k = Root then Failed
     (* check time of evict < current time *)
-    else if not (MHD.ts_lt clock t) then Failed
+    else if not (ts_lt clock t) then Failed
     (* check s was added through blum *)  
-    else if get_add_method_at st s <> V.BAdd then Failed
+    else if add_method_of st s <> Spec.BAdd then Failed
     (* check k has no children n the store *)
-    else if (
-              lemma_contains_key st s k;
-              has_instore_merkle_desc st k
-            ) then Failed  
+    else if has_instore_merkle_desc st k then Failed  
     else 
       (* update evict hash *)
       let h = thread_hevict vs in
-      let h_upd = MH.ms_hashfn_upd (MHD.MHDom (k,v) t (thread_id_of vs)) h in
+      let h_upd = ms_hashfn_upd (MHDom (k,v) t (thread_id_of vs)) h in
       let vs_upd = update_thread_hevict vs h_upd in
       (* update clock *)
       let vs_upd2 = update_thread_clock vs_upd t in    
       (* evict record *)
-      let st_upd = evict_record st s in
+      let st_upd = evict_from_store st s in
       update_thread_store vs_upd2 st_upd
 
-let vevictbm (s:slot_id) (k0:key) (s':slot_id) (k0':merkle_key) (t:timestamp) (vs:vtls {Valid? vs}): vtls = 
+let vevictbm (s:slot_id) (s':slot_id) (t:timestamp) (vs:vtls {Valid? vs}): vtls = 
   let st = thread_store vs in
   (* check store contains s and s' *)
-  if not (contains_record st s && contains_record st s') then Failed
+  if not (store_contains st s && store_contains st s') then Failed
   else
-    let k = get_key_at st s in
-    let k' = get_key_at st s' in
-    let v' = get_value_at st s' in
-    (* check keys are consistent with arguments *)
-    if k <> k0 then Failed
-    else if k' <> k0' then Failed
+    let k = stored_key st s in
+    let k' = stored_key st s' in
+    let v' = stored_value st s' in
     (* check k is a proper desc of k' *)
-    else if not (BT.is_proper_desc k k') then Failed
+    if not (is_proper_desc k k') then Failed
     (* check s was added through merkle *)
-    else if get_add_method_at st s <> V.MAdd then Failed  
+    else if add_method_of st s <> Spec.MAdd then Failed  
     (* check k has no children in the store *)
-    else if (
-              lemma_contains_key st s k;
-              has_instore_merkle_desc st k 
-            ) then Failed  
+    else if has_instore_merkle_desc st k then Failed  
     else
-      let v' = R.to_merkle_value v' in
-      let d = BT.desc_dir k k' in
-      let dh' = R.desc_hash_dir v' d in
+      // TODO: remove the assert with a better SMTPat for stored_value_matches_stored_key
+      let _ = assert (is_value_of k' v') in 
+      let v' = to_merkle_value v' in
+      let d = desc_dir k k' in
+      let dh' = desc_hash_dir v' d in
       match dh' with
-      | R.Empty -> Failed
-      | R.Desc k2 h2 b2 -> if k2 <> k || b2 then Failed
-                          else
-                            let v'_upd = V.update_merkle_value v' d k h2 true in
-                            let st_upd = update_record_value st s' (R.MVal v'_upd) in
-                            vevictb s k0 t (update_thread_store vs st_upd)
-
-(* thread-level verification step
-   (following the defn in Veritas.Verifier) *)
-let t_verify_step (vs:vtls)
-                  (e:logSK_entry): vtls =                           
-  match vs with
-  | Failed -> Failed (* could check the is_map flag here *)
-  | _ ->
-    match e with
-    | Get_SK s k v -> vget s k v vs
-    | Put_SK s k v -> vput s k v vs
-    | AddM_SK s r s' k'  -> vaddm s r s' k' vs
-    | EvictM_SK s k s' k' -> vevictm s k s' k' vs
-    | AddB_SK s r t j -> vaddb s r t j vs
-    | EvictB_SK s k t -> vevictb s k t vs
-    | EvictBM_SK s k s' k' t -> vevictbm s k s' k' t vs
-
-(* verify a log from a specified initial state *)
-let rec t_verify_aux (vs:vtls) (l:logSK): Tot vtls
-  (decreases (Seq.length l)) =
-  let n = Seq.length l in
-  if n = 0 then vs
-  else
-    let l' = SA.prefix l (n - 1) in
-    let vs' = t_verify_aux vs l' in
-    let e' = Seq.index l (n - 1) in
-    t_verify_step vs' e'
+      | Empty -> Failed
+      | Desc k2 h2 b2 -> 
+          if k2 <> k || b2 then Failed
+          else
+            let v'_upd = Spec.update_merkle_value v' d k h2 true in
+            let st_upd = update_store st s' (MVal v'_upd) in
+            vevictb s t (update_thread_store vs st_upd)
 
 // TODO: what should the initial size be?
-let empty_store:vstore = { data=Seq.create 10 None; is_map=true }
+let store_size = 65536 // 2 ^ 16
+let empty_store:vstore = { data=Seq.create store_size None; is_map=true }
 
-(* initialize verifier state *)
+(* Initialize verifier state *)
 let init_thread_state (id:thread_id): vtls = 
-  let vs = Valid id empty_store (MHD.MkTimestamp 0 0) MHD.empty_hash_value MHD.empty_hash_value in  
+  let vs = Valid id empty_store (MkTimestamp 0 0) empty_hash_value empty_hash_value in  
   if id = 0 then
     let st0 = thread_store vs in
-    let st0_upd = add_record st0 0 BT.Root (R.init_value BT.Root) V.MAdd in
+    let st0_upd = add_to_store st0 0 Root (init_value Root) Spec.MAdd in
     update_thread_store vs st0_upd    
   else vs
 
-let t_verify (id:thread_id) (l:logSK): vtls = 
-  t_verify_aux (init_thread_state id) l 
+let lemma_store_contains (st:vstore) (st':Spec.vstore) (s:slot_id) (k:key)
+  : Lemma (requires (store_rel st st' /\ slot_key_equiv st s k))
+          (ensures (store_contains st s = Spec.store_contains st' k))
+  = lemma_as_map_slot_key_equiv st s k
 
-let verify (id:thread_id) (l:logSK): vtls =
-  let vs = t_verify id l in
-  if Valid? vs
-  then if thread_store_is_map vs then vs else Failed
-  else Failed
+let lemma_stored_value (st:vstore) (st':Spec.vstore) (s:slot_id) (k:data_key)
+  : Lemma (requires (store_rel st st' /\ slot_key_equiv st s k))
+          (ensures (Spec.store_contains st' k /\ stored_value st s = Spec.stored_value st' k))
+  = lemma_as_map_slot_key_equiv st s k
 
-let verifiable (id:thread_id) (l: logSK): bool =
-  Valid? (verify id l)
-
-(** Proofs **)
-
-module Spec = Veritas.Verifier
-
-(* Relation between stores *)
-let store_rel (st:vstore) (st':Spec.vstore) : Type = 
-  st.is_map /\ FE.feq st' (as_map st)
-
-(* Relation between thread-local states *)
-let vtls_rel (vs:vtls) (vs':Spec.vtls) : Type =
-  match vs, vs' with
-  // either both runs failed
-  | Failed, Spec.Failed -> True
-  // or both are valid and the stores are related
-  | Valid id st clk ha he, Spec.Valid id' st' clk' _ ha' he' ->
-       store_rel st st' /\ 
-       // other fields related by equality  
-       id = id' /\ clk = clk' /\ ha = ha' /\ he = he'   
-  // or the spec run failed, but the store of vs is not a map
-  | Valid _ st _ _ _, _ -> not st.is_map
-  | _, _ -> False
-
-(* Relation between a slot and key *)
-let is_key_of (vs: vtls {Valid? vs}) (s:slot_id) (k:key) =
-  let st = thread_store vs in slot_key_equiv st s k
-
-let lemma_contains_record_store_contains 
-      (st:vstore) 
-      (s:slot_id) 
-      (st':Spec.vstore{store_rel st st'}) 
-      (k:key{slot_key_equiv st s k})
-  : Lemma (contains_record st s = Spec.store_contains st' k)
-  = admit()
-
-let lemma_get_value_at_stored_value
-      (st:vstore) 
-      (s:slot_id) 
-      (st':Spec.vstore{store_rel st st'}) 
-      (k:data_key{slot_key_equiv st s k /\ Spec.store_contains st' k})
-  : Lemma (get_value_at st s = Spec.stored_value st' k)
-  = admit()
-
-let lemma_update_record_value_update_store
-      (st:vstore) 
-      (s:slot_id) 
-      (st':Spec.vstore{store_rel st st'}) 
-      (k:data_key{slot_key_equiv st s k /\ Spec.store_contains st' k})
-      (v:data_value)
-  : Lemma (store_rel (update_record_value st s (R.DVal v)) (Spec.update_store st' k (R.DVal v)))
-  = admit()
+let lemma_update_store (st:vstore) (st':Spec.vstore) (s:slot_id) (k:data_key) (v:data_value)
+  : Lemma (requires (store_rel st st' /\ slot_key_equiv st s k))
+          (ensures (Spec.store_contains st' k /\
+                    store_rel (update_store st s (DVal v)) (Spec.update_store st' k (DVal v))))
+  = lemma_as_map_slot_key_equiv st s k;
+    admit()
 
 let lemma_vget_simulates_spec 
       (vs:vtls{Valid? vs})
@@ -394,12 +237,12 @@ let lemma_vget_simulates_spec
       (s:slot_id)
       (k:data_key)
       (v:data_value)
-  : Lemma (requires (vtls_rel vs vs' /\ is_key_of vs s k))
-          (ensures (vtls_rel (vget s k v vs) (Spec.vget k v vs')))
+  : Lemma (requires (vtls_rel vs vs' /\ slot_key_rel vs s k))
+          (ensures (vtls_rel (vget s v vs) (Spec.vget k v vs')))
   = let st = thread_store vs in
     let st' = Spec.thread_store vs' in
-    lemma_contains_record_store_contains st s st' k;
-    lemma_get_value_at_stored_value st s st' k
+    lemma_store_contains st st' s k;
+    lemma_stored_value st st' s k
 
 let lemma_vput_simulates_spec 
       (vs:vtls{Valid? vs}) 
@@ -407,22 +250,26 @@ let lemma_vput_simulates_spec
       (s:slot_id) 
       (k:data_key) 
       (v:data_value) 
-  : Lemma (requires (vtls_rel vs vs' /\ is_key_of vs s k))
-          (ensures (vtls_rel (vput s k v vs) (Spec.vput k v vs'))) 
+  : Lemma (requires (vtls_rel vs vs' /\ slot_key_rel vs s k))
+          (ensures (vtls_rel (vput s v vs) (Spec.vput k v vs'))) 
   = let st = thread_store vs in
     let st' = Spec.thread_store vs' in
-    lemma_contains_record_store_contains st s st' k;
-    lemma_update_record_value_update_store st s st' k v
+    lemma_store_contains st st' s k;
+    lemma_update_store st st' s k v
 
 let lemma_vaddm_simulates_spec 
       (vs:vtls{Valid? vs}) 
       (vs':Spec.vtls{Spec.Valid? vs'}) 
       (s s':slot_id)
-      (r:R.record)
+      (r:record)
       (k':merkle_key)  
-  : Lemma (requires (vtls_rel vs vs'))
-          (ensures (vtls_rel (vaddm s r s' k' vs) (Spec.vaddm r k' vs'))) 
-  = admit()
+  : Lemma (requires (vtls_rel vs vs') /\ slot_key_rel vs s' k')
+          (ensures (vtls_rel (vaddm s r s' vs) (Spec.vaddm r k' vs'))) 
+  = let st = thread_store vs in
+    let st' = Spec.thread_store vs' in
+    let (k,v) = r in
+    // ...
+    admit()
 
 let lemma_vevictm_simulates_spec 
       (vs:vtls{Valid? vs}) 
@@ -430,15 +277,15 @@ let lemma_vevictm_simulates_spec
       (s s':slot_id)
       (k:key)
       (k':merkle_key)  
-  : Lemma (requires (vtls_rel vs vs'))
-          (ensures (vtls_rel (vevictm s k s' k' vs) (Spec.vevictm k k' vs'))) 
+  : Lemma (requires (vtls_rel vs vs' /\ slot_key_rel vs s k /\ slot_key_rel vs s' k'))
+          (ensures (vtls_rel (vevictm s s' vs) (Spec.vevictm k k' vs'))) 
   = admit()
 
 let lemma_vaddb_simulates_spec 
       (vs:vtls{Valid? vs}) 
       (vs':Spec.vtls{Spec.Valid? vs'}) 
       (s:slot_id)
-      (r:R.record)
+      (r:record)
       (t:timestamp)
       (j:thread_id)
   : Lemma (requires (vtls_rel vs vs'))
@@ -451,8 +298,8 @@ let lemma_vevictb_simulates_spec
       (s:slot_id)
       (k:key)
       (t:timestamp)
-  : Lemma (requires (vtls_rel vs vs'))
-          (ensures (vtls_rel (vevictb s k t vs) (Spec.vevictb k t vs'))) 
+  : Lemma (requires (vtls_rel vs vs' /\ slot_key_rel vs s k))
+          (ensures (vtls_rel (vevictb s t vs) (Spec.vevictb k t vs'))) 
   = admit()
 
 let lemma_vevictbm_simulates_spec 
@@ -462,22 +309,15 @@ let lemma_vevictbm_simulates_spec
       (k:key)
       (k':merkle_key)
       (t:timestamp)
-  : Lemma (requires (vtls_rel vs vs'))
-          (ensures (vtls_rel (vevictbm s k s' k' t vs) (Spec.vevictbm k k' t vs'))) 
+  : Lemma (requires (vtls_rel vs vs' /\ slot_key_rel vs s k /\ slot_key_rel vs s' k'))
+          (ensures (vtls_rel (vevictbm s s' t vs) (Spec.vevictbm k k' t vs'))) 
   = admit()
 
-(* Relation between logs *)
-let log_rel  (l:logSK) (l':logK) : Type 
-  = skc l /\ drop_slots l = l'
-
-(* given a log with only slots, add consistent keys *)
-
-(* given a log with keys and slots, check that the key accesses are consistent with evicts and adds *)
-
+(*
 let lemma_t_verify_simulates_spec (id:thread_id) (l:logSK) (l':logK)
   : Lemma (requires (log_rel l l'))
           (ensures (vtls_rel (t_verify id l) (Spec.t_verify id l')))
-  = admit()
+  = 
 
 (* For any log, the intermediate implementation will verify 
    iff the the spec implementation does. *)
@@ -491,3 +331,4 @@ let lemma_verifiable_simulates_spec (id:thread_id) (l:logSK) (l':logK)
     if Valid? vs
     then if not (thread_store_is_map vs) 
     then admit()
+*)
