Veritas.Verifier.fst
@@ -244,7 +244,7 @@ let vaddm (r:record)
     | Desc k2 h2 b2 -> if k2 = k then
                          if h2 = h && b2 = false then
                            update_thread_store vs (add_to_store st k v MAdd)
-                         else Failed
+                          else Failed
                        else if v <> init_value k then Failed
                        else if not (is_proper_desc k2 k) then Failed
                        else
