intermediate/Veritas.Intermediate.StoreSKC.fst
@@ -1,0 +1,145 @@
+module Veritas.Intermediate.StoreSKC
+
+let get_slot (st:vstore) (s:slot_id)
+  : option vstore_entry
+  = if s >= Seq.length st.data then None 
+    else Seq.index st.data s
+
+let store_contains (st:vstore) (s:slot_id) : bool
+  = Some? (get_slot st s)
+
+let store_contains_st_index (st:vstore) (s:slot_id{store_contains st s})
+  : Lemma (s < Seq.length st.data)
+  = ()
+
+let stored_key (st:vstore) (s:slot_id{store_contains st s}) : key
+  = VStore?.k (Some?.v (get_slot st s))
+
+let stored_value (st:vstore) (s:slot_id{store_contains st s}) : value
+  = VStore?.v (Some?.v (get_slot st s))
+
+let stored_value_matches_stored_key (st:vstore) (s:slot_id{store_contains st s}) 
+  : Lemma (is_value_of (stored_key st s) (stored_value st s))
+  = ()
+
+let add_method_of (st:vstore) (s:slot_id{store_contains st s}) : add_method
+  = VStore?.am (Some?.v (get_slot st s))
+
+let lookup_key (st:vstore) (k:key) 
+  : option vstore_entry
+  = let f ro = if None? ro then false
+               else let Some r = ro in VStore?.k r = k in
+    let s = filter f st.data in
+    if Seq.length s = 0 then None
+    else Seq.index s 0 
+
+let store_contains_key (st:vstore) (k:key) : bool
+  = Some? (lookup_key st k)
+
+let lemma_lookup_key (st:vstore) (k:key) 
+  : Lemma (requires (store_contains_key st k))
+          (ensures (VStore?.k (Some?.v (lookup_key st k)) = k))
+  = let f ro = if None? ro then false
+               else let Some r = ro in VStore?.k r = k in
+    lemma_filter_correct1 f st.data 0
+
+let lemma_store_contains_key (st:vstore) (k:key)
+  : Lemma (requires (exists s. stored_key st s = k))
+          (ensures (store_contains_key st k))
+  = let f ro = if None? ro then false
+               else let Some r = ro in VStore?.k r = k in
+    lemma_filter_exists f st.data;
+    lemma_filter_correct1 f st.data 0
+
+let stored_value_by_key (st:vstore) (k:key{store_contains_key st k})
+  : value_type_of k
+  = lemma_lookup_key st k;
+    VStore?.v (Some?.v (lookup_key st k))
+
+let add_method_of_by_key (st:vstore) (k:key{store_contains_key st k})
+  : add_method
+  = VStore?.am (Some?.v (lookup_key st k))
+
+let update_slot (st:vstore) (s:st_index st) (e:vstore_entry)
+  : vstore
+  = { st with data = Seq.upd st.data s (Some e) }
+
+let update_store 
+  (st:vstore) 
+  (s:slot_id{store_contains st s}) 
+  (v:value_type_of (stored_key st s))
+  : Tot (st':vstore {store_contains st' s /\
+                     stored_value st' s = v})
+  = let Some (VStore k _ am) = get_slot st s in
+    update_slot st s (VStore k v am) 
+
+let update_store_preserves_length 
+      (st:vstore) 
+      (s:slot_id{store_contains st s}) 
+      (v:value_type_of (stored_key st s)) 
+  : Lemma (let st' = update_store st s v in
+           Seq.length st.data = Seq.length st'.data)
+  = ()
+
+let add_to_store 
+      (st:vstore) 
+      (s:st_index st) 
+      (k:key) 
+      (v:value_type_of k) 
+      (am:add_method)
+  : Tot (st':vstore {store_contains st' s /\
+                     stored_key st' s = k /\
+                     stored_value st' s = v /\
+                     add_method_of st' s = am})
+  = update_slot st s (VStore k v am)
+
+let evict_from_store (st:vstore) (s:st_index st)
+  : Tot (st':vstore {not (store_contains st' s)})
+  = { st with data = Seq.upd st.data s None }
+
+let rec as_map_aux (l:Seq.seq (option vstore_entry)) 
+  : Tot Spec.vstore (decreases (Seq.length l)) =
+  let n = Seq.length l in
+  if n = 0 then fun _ -> None
+  else 
+    let l' = prefix l (n - 1) in
+    let f' = as_map_aux l' in
+    match Seq.index l (n - 1) with
+    | None -> f'
+    | Some (VStore k v a) -> 
+      fun (k':key) -> if k = k' then Some (Spec.VStore v a) else f' k' 
+
+let as_map (st:vstore{st.is_map}) : Spec.vstore =
+  as_map_aux st.data
+
+let rec lemma_as_map_slot_key_equiv_aux 
+      (l:Seq.seq (option vstore_entry)) 
+      (s:seq_index l) 
+      (k:key) 
+      (v:value_type_of k) 
+      (am:add_method)
+  : Lemma (requires (Seq.index l s = Some (VStore k v am))) 
+          (ensures (Spec.store_contains (as_map_aux l) k /\
+                    Spec.stored_value (as_map_aux l) k = v))
+          (decreases (Seq.length l))
+  = let n = Seq.length l in
+    if n <> 0 
+    then
+      let l' = prefix l (n - 1) in
+      let f' = as_map_aux l' in
+      match Seq.index l (n - 1) with
+      | None -> lemma_as_map_slot_key_equiv_aux l' s k v am
+      | Some (VStore _ _ _) -> 
+          if s < n - 1 
+          then (
+                 lemma_as_map_slot_key_equiv_aux l' s k v am;
+                 // I thought the recursive call would work...
+                 admit()
+               )
+
+let lemma_as_map_slot_key_equiv (st:vstore{st.is_map}) (s:slot_id) (k:key)
+  : Lemma (requires (slot_key_equiv st s k)) 
+          (ensures (Spec.store_contains (as_map st) k /\
+                    stored_value st s = Spec.stored_value (as_map st) k)) 
+  = let Some (VStore k v a) = get_slot st s in 
+    lemma_as_map_slot_key_equiv_aux st.data s k v a
