intermediate/Veritas.Intermediate.StoreSKC.fsti
@@ -1,0 +1,89 @@
+module Veritas.Intermediate.StoreSKC
+
+open Veritas.Key
+open Veritas.Record
+open Veritas.SeqAux
+
+module Spec = Veritas.Verifier
+
+let slot_id = nat
+let add_method = Veritas.Verifier.add_method
+
+type vstore_entry = 
+  | VStore: k:key -> v:value_type_of k -> am:add_method -> vstore_entry
+
+type vstore = {
+  data:Seq.seq (option vstore_entry);
+  is_map:bool;
+}
+
+let st_index (st:vstore) = seq_index st.data
+
+val store_contains (st:vstore) (s:slot_id) : bool
+
+val store_contains_st_index (st:vstore) (s:slot_id{store_contains st s})
+  : Lemma (s < Seq.length st.data)
+          [SMTPat (store_contains st s)] 
+
+val stored_key (st:vstore) (s:slot_id{store_contains st s}) : key
+
+val stored_value (st:vstore) (s:slot_id{store_contains st s}) : value
+
+val stored_value_matches_stored_key (st:vstore) (s:slot_id{store_contains st s}) 
+  : Lemma (is_value_of (stored_key st s) (stored_value st s))
+    [SMTPat (is_value_of (stored_key st s) (stored_value st s))]
+
+val add_method_of (st:vstore) (s:slot_id{store_contains st s}) : add_method
+
+val store_contains_key (st:vstore) (k:key) : bool
+
+val lemma_store_contains_key (st:vstore) (k:key)
+  : Lemma (requires (exists s. stored_key st s = k))
+          (ensures (store_contains_key st k))
+          [SMTPat (store_contains_key st k)]
+
+val stored_value_by_key (st:vstore) (k:key{store_contains_key st k}) : value_type_of k
+
+val add_method_of_by_key (st:vstore) (k:key{store_contains_key st k}) : add_method
+
+val update_store 
+      (st:vstore) 
+      (s:slot_id{store_contains st s}) 
+      (v:value_type_of (stored_key st s))
+  : Tot (st':vstore {store_contains st' s /\
+                     stored_value st' s = v})
+
+val update_store_preserves_length 
+      (st:vstore) 
+      (s:slot_id{store_contains st s}) 
+      (v:value_type_of (stored_key st s)) 
+  : Lemma (let st' = update_store st s v in
+           Seq.length st.data = Seq.length st'.data)
+          [SMTPat (update_store st s v)]  
+
+val add_to_store 
+      (st:vstore) 
+      (s:st_index st) 
+      (k:key) 
+      (v:value_type_of k) 
+      (am:add_method)
+  : Tot (st':vstore {store_contains st' s /\
+                     stored_key st' s = k /\
+                     stored_value st' s = v /\
+                     add_method_of st' s = am})
+
+val evict_from_store (st:vstore) (s:st_index st)
+  : Tot (st':vstore {not (store_contains st' s)})
+
+(* slot_id s is equivalent to key k *)
+let slot_key_equiv (st:vstore) (s:slot_id) (k:key) : bool =
+  not st.is_map || // trivially true
+  (store_contains st s && stored_key st s = k) 
+
+(* convert a slot-indexed store to a key-indexed store *)
+val as_map (st:vstore{st.is_map}) : Spec.vstore
+
+val lemma_as_map_slot_key_equiv (st:vstore{st.is_map}) (s:slot_id) (k:key)
+  : Lemma (requires (slot_key_equiv st s k)) 
+          (ensures (Spec.store_contains (as_map st) k /\
+                    stored_value st s = Spec.stored_value (as_map st) k))
