intermediate/Veritas.Intermediate.VerifySKC.fsti
@@ -1,0 +1,241 @@
+module Veritas.Intermediate.VerifySKC
+
+open Veritas.Intermediate.Logs
+open Veritas.Intermediate.StoreSKC
+
+module FE = FStar.FunctionalExtensionality
+
+(* These are all independent of the 'verify' function; they should be safe to open *)
+open Veritas.BinTree
+open Veritas.Hash
+open Veritas.Key
+open Veritas.MultiSetHash
+open Veritas.MultiSetHashDomain
+open Veritas.Record
+open Veritas.SeqAux
+
+(* It's better not to open these modules to avoid naming conflicts *)
+module Spec = Veritas.Verifier
+module SpecT = Veritas.Verifier.Thread
+
+(* Thread-local state
+   id     : thread id
+   st     : thread local store
+   clock  : current timestamp
+   hadd   : add set hash
+   hevict : evict set hash *)
+noeq
+type vtls =
+  | Failed : vtls
+  | Valid :
+    id : thread_id ->
+    st : vstore ->
+    clock : timestamp ->
+    hadd : ms_hash_value ->
+    hevict : ms_hash_value ->
+    vtls
+
+let thread_id_of (vs:vtls {Valid? vs}): thread_id = 
+  Valid?.id vs
+
+let thread_store (vs: vtls {Valid? vs}): vstore =
+  Valid?.st vs
+
+let thread_store_is_map (vs: vtls {Valid? vs}): bool =
+  let st = thread_store vs in st.is_map
+
+let update_thread_store (vs:vtls {Valid? vs}) (st:vstore) : vtls =
+  match vs with
+  | Valid id _ clock hadd hevict -> Valid id st clock hadd hevict
+
+let thread_clock (vs:vtls {Valid? vs}) = 
+  Valid?.clock vs
+
+let update_thread_clock (vs:vtls {Valid? vs}) (clock:timestamp): vtls = 
+  match vs with
+  | Valid id st _ hadd hevict -> Valid id st clock hadd hevict
+
+let thread_hadd (vs:vtls {Valid? vs}) = 
+  Valid?.hadd vs
+
+let thread_hevict (vs:vtls {Valid? vs}) = 
+  Valid?.hevict vs
+
+let update_thread_hadd (vs:vtls {Valid? vs}) (hadd: ms_hash_value): vtls = 
+  match vs with
+  | Valid id st clock _ hevict -> Valid id st clock hadd hevict
+
+let update_thread_hevict (vs:vtls {Valid? vs}) (hevict:ms_hash_value): vtls = 
+  match vs with
+  | Valid id st clock hadd _ -> Valid id st clock hadd hevict
+
+val vget (s:slot_id) (v:data_value) (vs: vtls {Valid? vs}) : vtls 
+
+val vput (s:slot_id) (v:data_value) (vs: vtls {Valid? vs}) : vtls
+
+val vaddm (s:slot_id) (r:record) (s':slot_id) (vs: vtls {Valid? vs}): vtls 
+
+val vevictm (s:slot_id) (s':slot_id) (vs: vtls {Valid? vs}): vtls
+
+val vaddb (s:slot_id) (r:record) (t:timestamp) (j:thread_id) (vs:vtls {Valid? vs}): vtls
+
+val vevictb (s:slot_id) (t:timestamp) (vs:vtls {Valid? vs}): vtls
+
+val vevictbm (s:slot_id) (s':slot_id) (t:timestamp) (vs:vtls {Valid? vs}): vtls
+
+(* Note that the key values aren't used in the v* functions -
+   they are just useful (maybe?) for proof *)
+let t_verify_step (vs:vtls) (e:logSK_entry): vtls =
+  match vs with
+  | Failed -> Failed
+  | _ ->
+    match e with
+    | Get_SK s _ v -> vget s v vs
+    | Put_SK s _ v -> vput s v vs
+    | AddM_SK s r s' _  -> vaddm s r s' vs
+    | EvictM_SK s _ s' _ -> vevictm s s' vs
+    | AddB_SK s r t j -> vaddb s r t j vs
+    | EvictB_SK s _ t -> vevictb s t vs
+    | EvictBM_SK s _ s' _ t -> vevictbm s s' t vs
+
+(* Verify a log from a specified initial state *)
+let rec t_verify_aux (vs:vtls) (l:logSK): Tot vtls
+  (decreases (Seq.length l)) =
+  let n = Seq.length l in
+  if n = 0 then vs
+  else
+    let l' = prefix l (n - 1) in
+    let vs' = t_verify_aux vs l' in
+    let e' = Seq.index l (n - 1) in
+    t_verify_step vs' e'
+
+(* Main verify function *)
+val init_thread_state (id:thread_id): vtls
+
+let t_verify (id:thread_id) (l:logSK): vtls = 
+  t_verify_aux (init_thread_state id) l 
+
+let verify (id:thread_id) (l:logSK): vtls =
+  let vs = t_verify id l in
+  if Valid? vs
+  then if thread_store_is_map vs then vs else Failed
+  else Failed
+
+let verifiable (id:thread_id) (l: logSK): bool =
+  Valid? (verify id l)
+
+(* Relation between stores *)
+let store_rel (st:vstore) (st':Spec.vstore) : Type = 
+  st.is_map /\ FE.feq st' (as_map st)
+
+(* Relation between thread-local states *)
+let vtls_rel (vs:vtls) (vs':Spec.vtls) : Type =
+  match vs, vs' with
+  // either both runs failed
+  | Failed, Spec.Failed -> True
+  // or both are valid and the stores are related
+  | Valid id st clk ha he, Spec.Valid id' st' clk' _ ha' he' ->
+       store_rel st st' /\ 
+       // other fields related by equality  
+       id = id' /\ clk = clk' /\ ha = ha' /\ he = he'   
+  // or the spec run failed, but the store of vs is not a map
+  | Valid _ st _ _ _, _ -> not st.is_map
+  | _, _ -> False
+
+(* Relation between a slot and key *)
+let slot_key_rel (vs: vtls {Valid? vs}) (s:slot_id) (k:key) =
+  let st = thread_store vs in slot_key_equiv st s k
+
+val lemma_vget_simulates_spec 
+      (vs:vtls{Valid? vs})
+      (vs':Spec.vtls{Spec.Valid? vs'})
+      (s:slot_id)
+      (k:data_key)
+      (v:data_value)
+  : Lemma (requires (vtls_rel vs vs' /\ slot_key_rel vs s k))
+          (ensures (vtls_rel (vget s v vs) (Spec.vget k v vs')))
+
+val lemma_vput_simulates_spec 
+      (vs:vtls{Valid? vs}) 
+      (vs':Spec.vtls{Spec.Valid? vs'}) 
+      (s:slot_id) 
+      (k:data_key) 
+      (v:data_value) 
+  : Lemma (requires (vtls_rel vs vs' /\ slot_key_rel vs s k))
+          (ensures (vtls_rel (vput s v vs) (Spec.vput k v vs'))) 
+
+val lemma_vaddm_simulates_spec 
+      (vs:vtls{Valid? vs}) 
+      (vs':Spec.vtls{Spec.Valid? vs'}) 
+      (s s':slot_id)
+      (r:record)
+      (k':merkle_key)  
+  : Lemma (requires (vtls_rel vs vs') /\ slot_key_rel vs s' k')
+          (ensures (vtls_rel (vaddm s r s' vs) (Spec.vaddm r k' vs'))) 
+
+val lemma_vevictm_simulates_spec 
+      (vs:vtls{Valid? vs}) 
+      (vs':Spec.vtls{Spec.Valid? vs'}) 
+      (s s':slot_id)
+      (k:key)
+      (k':merkle_key)  
+  : Lemma (requires (vtls_rel vs vs' /\ slot_key_rel vs s k /\ slot_key_rel vs s' k'))
+          (ensures (vtls_rel (vevictm s s' vs) (Spec.vevictm k k' vs'))) 
+
+val lemma_vaddb_simulates_spec 
+      (vs:vtls{Valid? vs}) 
+      (vs':Spec.vtls{Spec.Valid? vs'}) 
+      (s:slot_id)
+      (r:record)
+      (t:timestamp)
+      (j:thread_id)
+  : Lemma (requires (vtls_rel vs vs'))
+          (ensures (vtls_rel (vaddb s r t j vs) (Spec.vaddb r t j vs')))
+
+val lemma_vevictb_simulates_spec 
+      (vs:vtls{Valid? vs}) 
+      (vs':Spec.vtls{Spec.Valid? vs'}) 
+      (s:slot_id)
+      (k:key)
+      (t:timestamp)
+  : Lemma (requires (vtls_rel vs vs' /\ slot_key_rel vs s k))
+          (ensures (vtls_rel (vevictb s t vs) (Spec.vevictb k t vs'))) 
+
+val lemma_vevictbm_simulates_spec 
+      (vs:vtls{Valid? vs}) 
+      (vs':Spec.vtls{Spec.Valid? vs'}) 
+      (s s':slot_id)
+      (k:key)
+      (k':merkle_key)
+      (t:timestamp)
+  : Lemma (requires (vtls_rel vs vs' /\ slot_key_rel vs s k /\ slot_key_rel vs s' k'))
+          (ensures (vtls_rel (vevictbm s s' t vs) (Spec.vevictbm k k' t vs'))) 
+
+(* Relation between logs -- haven't really worked this out yet *)
+let log_rel  (l:logSK) (l':logK) : Type 
+  = skc l /\ drop_slots l = l'
+
+// The property we want for log_rel:
+//   * l and l' have matching entries, and their keys & slots are related given 
+//     the state computed so far
+
+val lemma_init_thread_state_rel (id:thread_id) :
+  Lemma (vtls_rel (init_thread_state id) (Spec.init_thread_state id))
+
+let lemma_t_verify_simulates_spec (id:thread_id) (l:logSK) (l':logK)
+  : Lemma (requires (log_rel l l'))
+          (ensures (vtls_rel (t_verify id l) (Spec.t_verify id l')))
+  = admit()
+
+(* For any log, the intermediate implementation will verify 
+   iff the the spec implementation does. *)
+
+let lemma_verifiable_simulates_spec (id:thread_id) (l:logSK) (l':logK)
+  : Lemma (requires (log_rel l l'))
+          (ensures (let tl : SpecT.thread_id_vlog = (id,l') in
+                    verifiable id l = SpecT.verifiable tl))
+  = lemma_t_verify_simulates_spec id l l';
+    let vs = t_verify id l in
+    if Valid? vs
+    then if not (thread_store_is_map vs) 
+    then admit()
